mailbox/verif_mailbox_read.v
@@ -18,7 +18,7 @@ Proof.
   assert_PROP (Zlength reads = N) by entailer!.
   assert (0 <= r < N) as Hr.
   { exploit (Znth_inbounds r reads); [|lia].
-    intro Heq; rewrite Heq in *; contradiction. }
+    intro Heq; rewrite -> Heq in *; contradiction. }
   assert (N < Int.max_signed) by computable.
   forward.
   forward.
@@ -34,62 +34,52 @@ Proof.
   assert_PROP (Zlength reads = N) by entailer!.
   assert (0 <= r < N) as Hr.
   { exploit (Znth_inbounds r reads); [|lia].
-    intro Heq; rewrite Heq in *; contradiction. }
+    intro Heq; rewrite -> Heq in *; contradiction. }
   assert (N < Int.max_signed) by computable.
   forward.
-  rewrite comm_loc_isptr; Intros.
-  forward.
-  { entailer!. rewrite Znth_map; [auto|]. rewrite Zlength_map in *; simpl in *; lia. }
+(*  rewrite comm_loc_isptr; Intros. *)
   forward.
   forward.
   set (c := Znth r comms).
-  set (l := Znth r locks).
-  forward_call (sh2, c, g, l, vint 0, Empty, h,
-    fun h b => !!(b = Empty /\ latest_read h (vint b0)) &&
-      (EX v : Z, data_at sh tbuffer (vint v) (Znth b0 bufs)) * ghost_var gsh1 (vint b0) g0,
-    comm_R bufs sh gsh2 g0 g1 g2, fun h b => EX b' : Z, !!((if eq_dec b Empty then b' = b0 else b = vint b') /\
-      -1 <= b' < B /\ latest_read h (vint b')) &&
-      (EX v : Z, data_at sh tbuffer (vint v) (Znth b' bufs)) * ghost_var gsh1 (vint b') g0).
-  { entailer!. rewrite Znth_map; rewrite Zlength_map in *; auto; lia. }
+  forward_call AE_sub (sh2, c, g, vint 0, Empty, h,
+    fun h b => ⌜b = Empty /\ latest_read h (vint b0)⌝ ∧
+      (∃ v : Z, data_at sh tbuffer (vint v) (Znth b0 bufs)) ∗ ghost_frag (vint b0) g0,
+    comm_R bufs sh g0 g1 g2, fun h b => ∃ b' : Z, ⌜(if eq_dec b Empty then b' = b0 else b = vint b') /\
+      -1 <= b' < B /\ latest_read h (vint b')⌝ ∧
+      (∃ v : Z, data_at sh tbuffer (vint v) (Znth b' bufs)) ∗ ghost_frag (vint b') g0).
   { unfold comm_loc; entailer!.
-    rewrite <- emp_sepcon at 1; apply sepcon_derives; [|cancel].
-    unfold AE_spec.
-    apply allp_right; intro hc.
-    apply allp_right; intro hx.
-    apply allp_right; intro vc.
-    apply allp_right; intro vx.
-    rewrite <- imp_andp_adjoint; Intros.
-    rewrite <- wand_sepcon_adjoint, emp_sepcon; Intros.
-    unfold comm_R at 1 2.
-    rewrite !rev_app_distr; simpl.
-    rewrite !last_two_reads_cons, prev_taken_cons.
+    rewrite <- bi.emp_sep at 1; apply bi.sep_mono; last cancel.
+    rewrite /AE_spec.
+    iIntros "_" (???? (? & ? & Hincl)) "(>comm & (% & %) & buf & g0)".
+    rewrite /comm_R.
+    rewrite !rev_app_distr /= !last_two_reads_cons prev_taken_cons.
     unfold last_write in *; simpl in *.
     pose proof (last_two_reads_fst (rev hx)).
-    Intros b b1 b2.
-    assert (last_two_reads (rev hx) = (vint b1, vint b2)) as Hlast by assumption.
-    rewrite <- sepcon_assoc, sepcon_comm, <- !sepcon_assoc, 3sepcon_assoc.
-    erewrite ghost_var_share_join' by eauto; Intros.
-    eapply derives_trans; [apply sepcon_derives, derives_refl;
-      apply ghost_var_update with (v' := vint (if eq_dec (vint b) Empty then b0 else b))|].
-    eapply derives_trans, bupd_mono; [apply bupd_frame_r|].
+    iDestruct "comm" as (???) "(%Hcomm & a0 & a1 & a2 & buf')".
+    destruct Hcomm as (-> & ? & Hhx & Hlast & ? & ?).
+    iMod (ghost_var_update _ _ _ (vint (if eq_dec (vint b) Empty then b0 else b)) with "a0 g0") as "(%Heq & a0 & g0)".
     assert (repable_signed b0) by (apply repable_buf; lia).
-    assert (b1 = b0) by (apply repr_inj_signed; auto); subst.
+    assert (b1 = b0) as -> by (apply repr_inj_signed; auto; congruence).
     lapply (repable_buf b); auto; intro.
     rewrite Hlast.
-    erewrite <- ghost_var_share_join by eauto.
-    Exists (-1) (if eq_dec (vint b) Empty then b0 else b)
-      (if eq_dec (vint b) Empty then b2 else b0); entailer!.
+    iIntros "!>". rewrite -bi.later_intro.
+    rewrite bi.sep_exist_r; iExists (-1).
+    rewrite bi.sep_exist_r; iExists (if eq_dec (vint b) Empty then b0 else b).
+    rewrite bi.sep_exist_r; iExists (if eq_dec (vint b) Empty then b2 else b0).
+    iStopProof; entailer!.
     { split; [rewrite Forall_app; repeat constructor; auto|].
       { exists b, (-1); split; [|split]; auto; lia. }
-      rewrite eq_dec_refl.
+      split; last by if_tac.
+      if_tac; last done.
       if_tac; auto. }
-    rewrite !eq_dec_refl.
+    setoid_rewrite (if_true (Empty = Empty)); [|done..].
+    setoid_rewrite (if_true (-1 = -1)); [|done..].
     Exists (if eq_dec (vint b) Empty then b0 else b).
-    rewrite <- exp_sepcon2; cancel.
-    lapply (hist_incl_lt hc hx); auto; intro.
+    rewrite -!bi.sep_exist_l -!bi.sep_exist_r; cancel.
+    apply hist_incl_lt in Hincl; last done.
     destruct (eq_dec (vint b) Empty).
     - assert (b = -1) by (apply Empty_inj; auto; apply repable_buf; auto).
-      subst; rewrite eq_dec_refl; entailer!.
+      rewrite if_true //; entailer!.
       rewrite latest_read_Empty; auto.
     - destruct (eq_dec b (-1)); [subst; contradiction n; auto|].
       entailer!.
@@ -97,12 +87,12 @@ Proof.
   Intros x b'; destruct x as (t, v). simpl fst in *; simpl snd in *.
   assert (exists b, v = vint b /\ -1 <= b < B /\ if eq_dec b (-1) then b' = b0 else b' = b) as (b & ? & ? & ?).
   { destruct (eq_dec v Empty); subst.
-    - exists (-1); rewrite eq_dec_refl; split; auto; lia.
+    - exists (-1); if_tac; last done; split; auto; lia.
     - do 2 eexists; eauto; split; [lia|].
       destruct (eq_dec b' (-1)); [subst; contradiction n; auto | auto]. }
   exploit repable_buf; eauto; intro; subst.
   forward_if (temp _t'2 (bool2val (negb (eq_dec b (-1))))).
-  { if_tac in H13; try lia.
+  { destruct (eq_dec b (-1)); try lia; subst.
     forward.
     entailer!!.
     destruct (zlt _ _); auto.
@@ -112,31 +102,30 @@ Proof.
     entailer!!. }
   forward_if (PROP () LOCAL (temp _b (vint (if eq_dec b (-1) then b0 else b)); temp _rr (Znth r reads);
       temp _r (vint r); gvars gv)
-    SEP (comm_loc sh2 l c g g0 g1 g2 bufs sh gsh2 (map_upd h t (AE (vint b) Empty));
-         EX v : Z, data_at sh tbuffer (vint v) (Znth (if eq_dec b (-1) then b0 else b) bufs);
-         ghost_var gsh1 (vint b') g0;
+    SEP (comm_loc sh2 c g g0 g1 g2 bufs sh (<[t := Excl (AE (vint b) Empty)]>h);
+         ∃ v : Z, data_at sh tbuffer (vint v) (Znth (if eq_dec b (-1) then b0 else b) bufs);
+         ghost_frag (vint b') g0;
          data_at sh1 (tarray (tptr tint) N) reads (gv _reading); data_at sh1 (tarray (tptr tint) N) lasts (gv _last_read);
          data_at_ Ews tint (Znth r reads);
          data_at Ews tint (vint (if eq_dec b (-1) then b0 else b)) (Znth r lasts);
-         data_at sh1 (tarray (tptr tint) N) comms (gv _comm);
-         data_at sh1 (tarray (tptr t_lock) N) (map ptr_of locks) (gv _lock))).
-  -
-    forward. if_tac; inv H11.
+         data_at sh1 (tarray (tptr t_atom_int) N) comms (gv _comm))).
+  - forward.
+    destruct (eq_dec b (-1)); try done.
     entailer!!.
-  - forward. if_tac; inv H11.
+  - forward.
+    destruct (eq_dec b (-1)); try done.
     entailer!!.
   - forward.
     forward.
     Exists (if eq_dec b (-1) then b0 else b) t (vint b) v.
-    apply andp_right.
-    { apply prop_right.
-      split; [destruct (eq_dec b (-1)); auto; lia|].
+    entailer!!.
+    { split; [destruct (eq_dec b (-1)); auto; lia|].
       destruct (eq_dec (vint b) Empty).
       + assert (b = -1) by (apply Empty_inj; auto).
-        subst; rewrite eq_dec_refl; auto.
+        if_tac; try done; subst; auto.
       + destruct (eq_dec b (-1)); [subst; contradiction n; auto|].
-        split; auto; split; auto; apply latest_read_new; auto. }
-    subst c l; cancel.
+        split; auto; apply latest_read_new; auto. }
+    subst c; cancel.
     destruct (eq_dec b (-1)); subst; apply derives_refl.
 Qed.
 
@@ -147,7 +136,7 @@ Proof.
   assert_PROP (Zlength reads = N) by entailer!.
   assert (0 <= r < N) as Hr.
   { exploit (Znth_inbounds r reads); [|lia].
-    intro Heq; rewrite Heq in *; contradiction. }
+    intro Heq; rewrite -> Heq in *; contradiction. }
   assert (N < Int.max_signed) by computable.
   forward.
   forward.
