mailbox/verif_mailbox_reader.v
@@ -23,20 +23,18 @@ Proof.
   forward_call (r, reads, lasts, sh1, gv).
 (*  eapply semax_seq'; [|apply semax_ff]. *)
   set (c := Znth r comms).
-  set (l := Znth r locks).
-  forward_loop (EX b0 : Z, EX h : hist, PROP (0 <= b0 < B; latest_read h (vint b0))
+  forward_loop (∃ b0 : Z, ∃ h : hist, PROP (0 <= b0 < B; latest_read h (vint b0))
     LOCAL (temp _r (vint r); temp _arg arg; gvars gv)
     SEP (data_at sh1 (tarray (tptr tint) N) reads (gv _reading); data_at sh1 (tarray (tptr tint) N) lasts (gv _last_read);
          data_at Ews tint Empty (Znth r reads); data_at Ews tint (vint b0) (Znth r lasts);
          data_at Ews tint (vint r) (force_val (sem_cast_pointer arg)); malloc_token Ews tint arg;
-         data_at sh1 (tarray (tptr tint) N) comms (gv _comm);
-         data_at sh1 (tarray (tptr t_lock) N) (map ptr_of locks) (gv _lock);
+         data_at sh1 (tarray (tptr t_atom_int) N) comms (gv _comm);
          data_at sh1 (tarray (tptr tbuffer) B) bufs (gv _bufs);
-         comm_loc sh2 l c g g0 g1 g2 bufs sh gsh2 h;
-         EX v : Z, @data_at CompSpecs sh tbuffer (vint v) (Znth b0 bufs);
-         ghost_var gsh1 (vint b0) g0))
-  break: (@FF (environ->mpred) _).
-  { Exists 1 (empty_map : hist); entailer!.
+         comm_loc sh2 c g g0 g1 g2 bufs sh h;
+         ∃ v : Z, data_at sh tbuffer (vint v) (Znth b0 bufs);
+         ghost_frag (vint b0) g0)).
+(*  break: (@FF (environ->mpred) _). *)
+  { Exists 1 (∅ : hist); entailer!.
     unfold latest_read.
     left; split; auto; discriminate. }
   Intros b0 h.
